Caching implementation work.

src/BinEncoders/Env/Lib2/DomainNameOpt.v
@@ -25,7 +25,70 @@ Section DomainName.
 
   (* The terminal character for domain names is the byte of all zeros. *)
   Definition terminal_char : ascii := zero.
-  Definition pointerT := ({w : word 8 | wlt (natToWord 8 191) w} * word 8)%type.
+  Definition pointerT := (sig (wlt (natToWord 8 191)) * word 8)%type.
+  Definition pointerT2Nat (p : pointerT) : nat :=
+    (wordToNat (projT1 (fst p)) * 256) + wordToNat (snd p).
+
+  Lemma Nat2pointerT_pf :
+    forall n,
+      natToWord 8 191 < natToWord 8 (NPeano.modulo (NPeano.div n 256) 64 + 192).
+  Proof.
+    intros; apply WordFacts.natToWord_wlt.
+    - simpl; apply Nomega.Nlt_in; simpl; compute; omega.
+    - apply Nomega.Nlt_in.
+      apply Lt.lt_le_trans with (m := 64 + 192);
+        [ rewrite Nnat.Nat2N.id | compute; omega].
+      apply Plus.plus_lt_compat_r.
+      refine (proj2 (NPeano.mod_bound_pos _ _ _ _)); omega.
+    - omega.
+  Qed.
+
+  Lemma div_eq: forall a b : nat,
+      b <> 0
+      -> b * NPeano.div a b = a - NPeano.modulo a b.
+  Proof.
+    intros; rewrite NPeano.Nat.mod_eq by assumption.
+    rewrite sub_plus; try omega.
+    apply NPeano.Nat.mul_div_le; auto.
+  Qed.
+
+  Definition Nat2pointerT (n : nat) : pointerT :=
+    (exist _ _ (Nat2pointerT_pf n),
+     natToWord 8 (NPeano.modulo n 256)).
+
+  Lemma Nat2pointerT_pointerT2Nat :
+    forall p, Nat2pointerT (pointerT2Nat p) = p.
+  Proof.
+    destruct p as [[upper_p upper_p_OK] lower_p].
+    unfold pointerT2Nat; simpl.
+    unfold Nat2pointerT; f_equal.
+    assert ((natToWord 8 (NPeano.modulo (NPeano.div (wordToNat upper_p * 256 + wordToNat lower_p) 256) 64 + 192)) = upper_p).
+    - rewrite NPeano.Nat.div_add_l; auto with arith.
+      rewrite NPeano.Nat.div_small, NPeano.Nat.add_0_r.
+      rewrite NPeano.Nat.mod_eq by omega.
+      replace (64 * NPeano.div (wordToNat upper_p) 64) with 192.
+      rewrite NPeano.Nat.sub_add.
+      apply natToWord_wordToNat.
+      apply WordFacts.wordToNat_lt in upper_p_OK; eauto.
+      rewrite div_eq by omega.
+      apply WordFacts.wordToNat_lt in upper_p_OK; simpl in upper_p_OK.
+      revert upper_p_OK; clear.
+      shatter_word upper_p.
+      abstract (destruct x; destruct x0; destruct x1; destruct x2;
+                destruct x3; destruct x4; destruct x5; destruct x6; simpl;
+                intro; try omega).
+      apply wordToNat_bound.
+    - generalize (Nat2pointerT_pf (wordToNat upper_p * 256 + wordToNat lower_p));
+        rewrite H; intros.
+      f_equal.
+      apply UIP_dec.
+      decide equality.
+    - rewrite Plus.plus_comm, NPeano.Nat.mod_add by omega.
+      rewrite NPeano.Nat.mod_eq by omega.
+      rewrite NPeano.Nat.div_small by apply wordToNat_bound.
+      simpl mult; rewrite <- Minus.minus_n_O.
+      apply natToWord_wordToNat.
+  Qed.
 
   Lemma terminal_char_eq :
     forall x0, terminal_char = ascii_of_N (wordToN x0)
@@ -41,7 +104,7 @@ Section DomainName.
   Qed.
 
   Context {cacheGet : CacheGet cache string pointerT}.
-  Context {cachePeek : CachePeek cache pointerT}.
+  Context {cachePeek : CachePeek cache (option pointerT)}.
   Definition add_ptr_OK
              (t : string * pointerT)
              (ce : CacheEncode)
@@ -82,20 +145,24 @@ Section DomainName.
              (`(ptr1b, env') <- encode_word_Spec (proj1_sig (fst position)) env;
               `(ptr2b, env') <- encode_word_Spec (snd position) env';
               ret (transform ptr1b ptr2b, env'))
-             Else (`(label, domain') <- { labeldomain' |
-                                          (domain = (fst labeldomain') ++ String "." (snd labeldomain') \/ labeldomain' = (domain, ""))
-                                          /\ ValidLabel (fst labeldomain')
-                                          /\ (forall label' post',
-                                                 domain = label' ++ post'
-                                                 -> ValidLabel label'
-                                                 -> String.length label' <= String.length (fst labeldomain'))}%string%nat;
-                     `(lenb, env') <- encode_nat_Spec 8 (String.length label) env;
-                     `(labelb, env') <- encode_string_Spec label env';
-                     `(domainb, env') <- encode_DomainName_Spec domain' env';
-                     ret (transform (transform lenb labelb) domainb, addE_G env' (domain, peekE env))))) domain env.
+    Else
+    (`(label, domain') <- { labeldomain' |
+                            (domain = (fst labeldomain') ++ String "." (snd labeldomain') \/ labeldomain' = (domain, ""))
+                            /\ ValidLabel (fst labeldomain')
+                            /\ (forall label' post',
+                                   domain = label' ++ post'
+                                   -> ValidLabel label'
+                                   -> String.length label' <= String.length (fst labeldomain'))}%string%nat;
+       `(lenb, env') <- encode_nat_Spec 8 (String.length label) env;
+       `(labelb, env') <- encode_string_Spec label env';
+       `(domainb, env') <- encode_DomainName_Spec domain' env';
+       ret (transform (transform lenb labelb) domainb,
+            (* If the pointer would overflow, don't record *)
+            Ifopt peekE env as curPtr Then addE_G env' (domain, curPtr)
+                                      Else env'
+      )))) domain env.
 
   (* Decode now uses a measure on the length of B *)
-
   Lemma lt_B_trans :
     forall b
            (b1 : {b' : B | le_B b' b})
@@ -105,6 +172,7 @@ Section DomainName.
     intros; destruct b1; destruct b3; simpl in *.
     unfold le_B, lt_B in *; omega.
   Qed.
+
 
   Lemma n_eq_0_lt :
     forall n,
@@ -170,7 +238,7 @@ Section DomainName.
     injection H; intros; eauto.
   Qed.
 
-    Lemma index_correct'
+  Lemma index_correct'
     : forall s a n,
       index 0 (String a EmptyString) s = Some n
       -> exists s' s'',
@@ -371,9 +439,13 @@ Section DomainName.
               Ifopt (index 0 "." label) as _ Then None
               Else (`(domain, b4, e3) <- rec (proj1_sig b3) (lt_B_trans _ _ _) env';
               If (string_dec domain "") Then
-                 Some (label, b4, addD_G e3 (label, peekD cd))
+                 Some (label, b4,
+                       Ifopt (peekD cd) as curPtr Then addD_G e3 (label, curPtr)
+                                                  Else e3)
                  Else Some (label ++ (String "." domain), b4,
-                            addD_G e3 (label ++ (String "." domain), peekD cd))
+                            Ifopt (peekD cd) as curPtr Then
+                            addD_G e3 (label ++ (String "." domain), curPtr)
+                            Else e3)
              )) end)
          Else None) end)%string b env);
     try exact decode_word_le;
@@ -407,9 +479,13 @@ Section DomainName.
                     Else (
                    `(domain, b4, e3) <- f (` b3) (lt_B_trans x b1 b3) env'0;
                    If (string_dec domain "") Then
-                      Some (label, b4, addD_G e3 (label, peekD cd))
+                      Some (label, b4,
+                            Ifopt (peekD cd) as curPtr Then addD_G e3 (label, curPtr)
+                                                       Else e3)
                    Else Some (label ++ (String "." domain), b4,
-                            addD_G e3 (label ++ (String "." domain), peekD cd)))%string
+                              Ifopt (peekD cd) as curPtr Then addD_G e3
+                                                         (label ++ (String "." domain), curPtr)
+                                                         Else e3))%string
                end Else None) end) =
    (fun cd : CacheDecode =>
       `(labelheader, b1, env') <- Decode_w_Measure_le decode_word x cd decode_word_le;
@@ -434,9 +510,12 @@ Section DomainName.
                      Else (
                      `(domain, b4, e3) <- g (` b3) (lt_B_trans x b1 b3) env'0;
                        If (string_dec domain "") Then
-                          Some (label, b4, addD_G e3 (label, peekD cd))
+                          Some (label, b4, Ifopt (peekD cd) as curPtr Then addD_G e3 (label, curPtr)
+                                                                                 Else e3)
                        Else Some (label ++ (String "." domain), b4,
-                                  addD_G e3 (label ++ (String "." domain), peekD cd)))%string
+                                  Ifopt (peekD cd) as curPtr Then addD_G e3
+                                                             (label ++ (String "." domain), curPtr)
+                                                             Else e3))%string
                end Else None) end).
   Proof.
     intros; apply functional_extensionality; intros.
@@ -480,7 +559,8 @@ Section DomainName.
                      `(domainb, env'1) <- rec domain' env'0;
                      ret
                        (transform (transform lenb labelb) domainb,
-                       addE_G env'1 (domain, peekE env0)))))
+                        Ifopt peekE env0 as curPtr Then addE_G env'1 (domain, curPtr)
+                                      Else env'1))))
    (fun (domain : DomainName) (env0 : CacheEncode) =>
     If string_dec domain "" Then encode_ascii_Spec terminal_char env0
     Else (
@@ -505,7 +585,8 @@ Section DomainName.
                      `(domainb, env'1) <- rec' domain' env'0;
                      ret
                        (transform (transform lenb labelb) domainb,
-                       addE_G env'1 (domain, peekE env0))))).
+                        Ifopt peekE env0 as curPtr Then addE_G env'1 (domain, curPtr)
+                                      Else env'1)))).
   Proof.
     simpl; intros; unfold Bind2.
     apply General.refine_if; intros; rewrite H0; simpl.
@@ -646,11 +727,12 @@ Section DomainName.
     apply UIP_dec.
     decide equality.
   Qed.
-  
+
   Variable add_peekD_OK :
-    forall domain ce cd,
+    forall domain ce cd n,
       Equiv ce cd
-      -> add_ptr_OK (domain, peekD cd) ce cd.
+      -> peekD cd = Some n
+      -> add_ptr_OK (domain, n) ce cd.
   Variable IndependentCaches :
     forall env p (b : nat),
       getD (addD env b) p = getD env p.
@@ -658,19 +740,33 @@ Section DomainName.
     forall env l p p',
       p <> p'
       -> getD (addD_G env (l, p)) p' = getD env p'.
+  Variable addPeekSome :
+    forall env n m,
+      peekD env = Some m
+      -> (n + (pointerT2Nat m) < pow2 14)%nat
+      -> exists p', peekD (addD env n) = Some p'
+                    /\ pointerT2Nat p' = n + (pointerT2Nat m).
+  Variable addPeekNone :
+    forall env n,
+      peekD env = None
+      -> peekD (addD env n) = None.
+  Variable addPeekNone' :
+    forall env n m,
+      peekD env = Some m
+      -> ~ (n + (pointerT2Nat m) < pow2 14)%nat
+      -> peekD (addD env n) = None.
+
   Variable addZeroPeek :
     forall xenv,
       peekD xenv = peekD (addD xenv 0).
-  Variable addPeek_eq :
-    forall xenv xenv' sz sz',
-      peekD xenv = peekD (addD xenv' (S sz'))
-      -> peekD xenv' <> peekD (addD xenv sz).
-  
+
+  Arguments pow2 : simpl never.
+
   Lemma decode_word_add_ptr_OK
-    : forall sz env xenv xenv' env' b b' x x1 l,
-      add_ptr_OK (l, peekD xenv') env xenv
-      -> decode_word (sz := sz) b xenv = Some (x, b', x1) 
-      -> add_ptr_OK (l, peekD xenv') env' x1.
+    : forall sz env xenv n env' b b' x x1 l,
+      add_ptr_OK (l, n) env xenv
+      -> decode_word (sz := sz) b xenv = Some (x, b', x1)
+      -> add_ptr_OK (l, n) env' x1.
   Proof.
     intros.
     unfold decode_word in H0.
@@ -679,12 +775,12 @@ Section DomainName.
     unfold add_ptr_OK.
     rewrite IndependentCaches; eauto.
   Qed.
-  
+
   Lemma decode_string_add_ptr_OK
-    : forall n env xenv xenv' xenv'' b b' l l',
-      add_ptr_OK (l', peekD xenv') env xenv 
+    : forall n env xenv n' xenv'' b b' l l',
+      add_ptr_OK (l', n') env xenv
       -> decode_string n b xenv = Some (l, b', xenv'')
-      -> add_ptr_OK (l', peekD xenv') env xenv''.
+      -> add_ptr_OK (l', n') env xenv''.
   Proof.
     unfold add_ptr_OK in *; induction n; simpl; intros.
     - injections; eauto.
@@ -700,7 +796,23 @@ Section DomainName.
       destruct (decode_word' 8 b); simpl in *; try discriminate; injections.
       rewrite IndependentCaches; eauto.
   Qed.
-  
+
+  Lemma addPeek :
+    forall env n m,
+      peekD env = Some m
+      -> peekD (addD env n) = Some (Nat2pointerT (n + (pointerT2Nat m)))
+         \/ peekD (addD env n) = None.
+  Proof.
+    intros;
+      destruct (Compare_dec.lt_dec (n + pointerT2Nat m) (pow2 14)).
+    - left; eapply addPeekSome in H; eauto.
+      destruct H as [p' [H' H''] ].
+      rewrite H', <- H''.
+      f_equal.
+      rewrite Nat2pointerT_pointerT2Nat; reflexivity.
+    - right; eapply addPeekNone' in H; eauto.
+  Qed.
+
   Lemma decode_word_peek_distinct
     : forall sz xenv xenv' b b' x,
       decode_word (sz := sz) b xenv = Some (x, b', xenv')
@@ -712,7 +824,7 @@ Section DomainName.
     injections.
     reflexivity.
   Qed.
-  
+
   Lemma decode_string_peek_distinct
     : forall n xenv xenv' b b' l,
       decode_string n b xenv = Some (l, b', xenv')
@@ -724,13 +836,43 @@ Section DomainName.
         destruct H as [? [? [? [? ?] ] ] ]; injections; subst.
       destruct (decode_string n x0 x1) eqn: ?; simpl in *; try discriminate.
       destruct p; destruct p; injections.
-      apply IHn in Heqo.
       unfold decode_ascii in H.
       apply DecodeBindOpt2_inv in H;
         destruct H as [? [? [? [? ?] ] ] ]; injections; subst.
       eapply decode_word_peek_distinct in H; eauto.
-      rewrite Heqo.
-  Admitted.      
+      eapply IHn in Heqo; eauto; rewrite Heqo.
+      destruct (peekD xenv) eqn: peekD_eq.
+      + destruct (Compare_dec.lt_dec (8 + (8 * n) + pointerT2Nat p) (pow2 14)).
+        * destruct (addPeekSome _ 8 _ peekD_eq) as [p' [? ?] ]; try omega.
+          rewrite H0 in H.
+          destruct (addPeekSome _ (8 * n) _ H) as [p'' [? ?] ]; try omega.
+          destruct (addPeekSome _ (8 * (S n)) _ peekD_eq) as [p''' [? ?] ]; try omega.
+          simpl in H4; rewrite H4.
+          rewrite H1 in H3.
+          simpl in H2; rewrite H2.
+          f_equal.
+          rewrite <- Nat2pointerT_pointerT2Nat, H5.
+          rewrite <- (Nat2pointerT_pointerT2Nat p''), H3.
+          f_equal.
+          omega.
+        * destruct (Compare_dec.lt_dec (8 + pointerT2Nat p) (pow2 14)).
+          { destruct (addPeekSome _ 8 _ peekD_eq) as [p' [? ?] ]; try omega.
+            erewrite !addPeekNone'; eauto.
+            omega.
+            rewrite H0 in H; eauto.
+            rewrite H1.
+            omega.
+          }
+          { rewrite addPeekNone; auto.
+            erewrite !addPeekNone'; eauto.
+            omega.
+            rewrite H.
+            eapply addPeekNone'; eauto.
+          }
+      + rewrite !addPeekNone; auto.
+        rewrite H.
+        apply addPeekNone; eauto.
+  Qed.
 
   Theorem DomainName_decode_correct
           (P_OK :
@@ -743,7 +885,6 @@ Section DomainName.
                     -> ValidDomainName domain /\ (String.length domain > 0)%nat)
                   /\ (forall env p domain,
                          P env
-
                          -> (ValidDomainName domain /\ String.length domain > 0)%nat
                          -> P (addD_G env (domain, p)))
                   /\ (forall (b : nat) (cd : CacheDecode),
@@ -753,7 +894,7 @@ Section DomainName.
     encode_decode_correct_f
       cache transformer
       (fun domain => ValidDomainName domain)
-      (fun s b => lt (String.length s + bin_measure b) (pow2 14))
+      (fun s b => True)
       encode_DomainName_Spec decode_DomainName cache_inv.
   Proof.
     unfold encode_decode_correct_f; split.
@@ -778,19 +919,22 @@ Section DomainName.
             Then match weq labelheader (wzero 8) with
                  | in_left => Some (""%string, ` b1, env')
                  | right n =>
-                     `(label, b3, env'0) <- Decode_w_Measure_lt 
-                                              (decode_string (wordToNat labelheader)) 
-                                              (` b1) env' 
+                     `(label, b3, env'0) <- Decode_w_Measure_lt
+                                              (decode_string (wordToNat labelheader))
+                                              (` b1) env'
                                               (decode_string_lt (wordToNat labelheader) (n_eq_0_lt labelheader n));
                      Ifopt index 0 "." label as _ Then None
                      Else (`(domain, b4, e3) <- rec (` b3) (lt_B_trans b0 b1 b3) env'0;
-                           If string_dec domain "" Then 
-                           Some (label, b4, addD_G e3 (label, peekD cd))
+                           If string_dec domain "" Then
+                              Some (label, b4,
+                                    Ifopt (peekD cd) as curPtr Then addD_G e3 (label, curPtr)
+                                                               Else e3)
                            Else Some
-                                  ((label ++ String "." domain)%string, b4,
-                                  addD_G e3 ((label ++ String "." domain)%string, peekD cd)))
+                           ((label ++ String "." domain)%string, b4,
+                            Ifopt (peekD cd) as curPtr Then addD_G e3 ((label ++ String "." domain)%string, curPtr)
+                                                       Else e3))
                  end Else None
-        end) (transform l' ext) xenv = Some (l, ext, xenv'0) /\ 
+        end) (transform l' ext) xenv = Some (l, ext, xenv'0) /\
      Equiv xenv' xenv'0 /\ True).
       simpl in *.
       generalize dependent l';
@@ -912,7 +1056,7 @@ Section DomainName.
                 reflexivity.
               + repeat apply add_correct; eauto.
               (* + erewrite peek_correct by eauto.
-                unfold add_ptr_OK; rewrite !IndependentCaches; eauto. 
+                unfold add_ptr_OK; rewrite !IndependentCaches; eauto.
                 eapply add_peekD_OK; eauto. *)
             }
           { (* Encoder did not to compress *)
@@ -924,7 +1068,7 @@ Section DomainName.
             generalize l_eq; intros [l_eq' | l_eq'].
             destruct (fun H => proj1 (Nat_decode_correct (P := fun _ => True) 8 (fun _ _ _ => I)) _ _ _ _ _ (transform b'' (transform b3 ext0)) Eeq H I Penc'') as [xenv4 [? xenv_eqv] ].
             pose proof ((proj1 Valid_data) ""%string label1 _ l_eq' label1_OK).
-            simpl; omega.
+            unfold pow2; omega.
             destruct (fun H => proj1 (String_decode_correct (P := fun _ => True) (fun _ _ _ => I) (String.length label1)) _ _ _ _ _ (transform b3 ext0) xenv_eqv H I Penc''') as [xenv6 [? xenv6_eqv] ]; eauto.
                 eapply IHn in Penc''''.
                 destruct Penc'''' as [xenv7 [? ?] ].
@@ -937,63 +1081,210 @@ Section DomainName.
               simpl in H4;
                 unfold decode_word at 1 in H4.
               rewrite <- !transform_assoc in H4.
-                  unfold decode_nat in H0.
+              unfold decode_nat in H0.
+              apply DecodeBindOpt2_inv in H0;
+                destruct H0 as [? [? [? [? ?] ] ] ]; injections; subst.
+              unfold decode_word in H0.
+              destruct (decode_word' 8 (transform b' (transform b'' (transform b3 ext0)))); simpl in H0; try discriminate; injections.
+              simpl in H4.
+              destruct (H4 _ _ _ (eq_refl _)).
+              rewrite <- !transform_assoc, H0; simpl; clear H0.
+              pose proof ((proj1 Valid_data) ""%string label1 _ (eq_refl _) label1_OK) as w';
+                rewrite H8 in w'.
+              destruct (wlt_dec WO~1~0~1~1~1~1~1~1 x); simpl;
+                try (elimtype False;
+                     apply WordFacts.wordToNat_lt in w; simpl in w; omega).
+              destruct (wlt_dec x WO~0~1~0~0~0~0~0~0); simpl.
+              * destruct (weq x (wzero 8)).
+                subst; simpl in H8.
+                destruct label1; simpl in H8; try discriminate.
+                unfold ValidLabel in label1_OK; simpl in label1_OK; omega.
+                match goal with
+                  |- context [Decode_w_Measure_lt ?x ?y ?z ?m] =>
+                  pose proof (Decode_w_Measure_lt_eq x y z m)
+                end.
+                simpl in H0; rewrite H8 in H1; rewrite H1 in H0.
+                destruct (H0 _ _ _ (eq_refl _)).
+                rewrite H5; simpl; rewrite H2.
+                destruct label1_OK as [H6' _]; rewrite H6';
+                  simpl.
+                destruct (string_dec label2 ""); simpl;
+                  try reflexivity.
+                generalize (proj2 Valid_data label1 label2 (eq_refl _)); intros;
+                  rewrite e in H6; intuition.
+              * destruct n2.
+                rewrite <- natToWord_wordToNat;
+                  rewrite <- (natToWord_wordToNat x).
+                apply WordFacts.natToWord_wlt.
+                simpl.
+                apply Nomega.Nlt_in.
+                rewrite Nnat.Nat2N.id; etransitivity; eauto.
+                simpl. unfold BinPos.Pos.to_nat; simpl.
+                revert w' n1; clear.
+                intros; omega.
+                apply Nomega.Nlt_in.
+                simpl. unfold BinPos.Pos.to_nat; simpl.
+                revert w' n1; clear; intros; omega.
+                revert w' n1; clear; intros; simpl; omega.
+            + split.
+              erewrite l_eq', peek_correct by eauto.
+              destruct (peekD xenv) eqn: peekD_eq.
+              simpl; apply add_correct_G; eauto.
+              intuition.
+              apply DecodeBindOpt2_inv in H0;
+                destruct H0 as [? [? [? [? ?] ] ] ]; injections; subst.
+              pose proof (decode_word_peek_distinct _ _ _ _ _ _ H0) as P.
+              pose proof (decode_string_peek_distinct _ _ _ _ _ _ H1) as P'.
+              eapply decode_word_add_ptr_OK in H0; eauto.
+              eapply decode_string_add_ptr_OK in H1; eauto.
+              assert (forall p', peekD xenv6 = Some p'
+                                 -> (pointerT2Nat p < pointerT2Nat p')%nat) as P3
+                  by (clear; admit).
+              unfold add_ptr_OK in *; simpl in *; revert addPeekSome addPeekNone addPeekNone' getDistinct IndependentCaches H2 H1 P P' P3; generalize xenv env p peekD_eq ; clear.
+              generalize (transform b3 ext0); intros b xenv env p peekD_eq.
+              revert label2 xenv6 xenv7 ext0 x1.
+              generalize env xenv (String.length label1); clear.
+              eapply (@well_founded_induction _ _ well_founded_lt_b) with
+              (a := b); intros.
+              rewrite Coq.Init.Wf.Fix_eq in H2; auto using decode_body_monotone; simpl.
+              apply DecodeBindOpt2_inv in H2;
+                destruct H2 as [? [? [? [? ?] ] ] ]; injections; subst.
+              destruct (wlt_dec  WO~1~0~1~1~1~1~1~1 x0); simpl in H2.
+              * (* The decoded word was a pointer. *)
+                symmetry in H2; apply DecodeBindOpt2_inv in H2;
+                  destruct H2 as [? [? [? [? ?] ] ] ]; injections; subst.
+                match type of H3 with
+                | context [getD ?env' ?w] => destruct (getD env' w) eqn:getD_eq;
+                                               try discriminate
+                end.
+                destruct s; try discriminate; injections.
+                eapply Decode_w_Measure_le_eq' in H2.
+                eapply Decode_w_Measure_le_eq' in H0.
+                unfold decode_word in H0.
+                destruct (decode_word' 8 x); simpl in *; try discriminate; injections.
+                unfold decode_word in H2.
+                destruct (decode_word' 8 (projT1 x2)); simpl in *; try discriminate; injections.
+                repeat match type of H2 with
+                       | context [dequeue_opt ?b] => destruct (dequeue_opt b) as [ [? ?] | ]; simpl in H2; try discriminate
+                       end.
+                injections.
+                rewrite !IndependentCaches; eauto.
+                repeat match type of H2 with
+                       | context [dequeue_opt ?b] => destruct (dequeue_opt b) as [ [? ?] | ]; simpl in H2; try discriminate
+                       end.
+                injections.
+                rewrite !IndependentCaches; eauto.
+                eauto.
+                eauto.
+              * destruct (wlt_dec x0 WO~0~1~0~0~0~0~0~0); simpl in H2; try discriminate.
+                destruct (weq x0 (wzero 8)); simpl in H2.
+                injections.
+                eapply Decode_w_Measure_le_eq' in H0.
+                unfold decode_word in H0.
+                destruct (decode_word' 8 x); simpl in *; try discriminate; injections.
+                rewrite IndependentCaches; eauto.
+                eauto.
+                symmetry in H2; apply DecodeBindOpt2_inv in H2;
+                  destruct H2 as [? [? [? [? ?] ] ] ]; injections; subst.
+                destruct (index 0 "." x4); simpl in H3; try discriminate.
+                match type of H3 with
+                | context [Fix well_founded_lt_b ?H' ?H0' ?H1' ?H2' ] =>
+                  destruct (Fix well_founded_lt_b H' H0' H1' H2') as [ [ [? ?] ?] | ] eqn:rec; simpl in H3;
+                    try discriminate
+                end.
+                eapply Decode_w_Measure_le_eq' in H0; eauto.
+                eapply Decode_w_Measure_lt_eq' in H2; eauto.
+                pose proof (decode_word_peek_distinct _ _ _ _ _ _ H0) as P''.
+                pose proof (decode_string_peek_distinct _ _ _ _ _ _ H2) as P'''.
+                assert (getD x6 p = None) by
+                    (revert H0 H2 H1 env; clear; intros;
+                     eapply decode_word_add_ptr_OK with (env := env) (env' := env) in H0; eauto;
+                     eapply decode_string_add_ptr_OK with (env := env) in H2; eauto).
+                simpl in P'''.
+                destruct (string_dec d ""); simpl in H3; injections;
+                  eapply (H) with (x1 := x3) (xenv := xenv6) in rec; eauto using lt_B_trans.
+                destruct (peekD xenv6) eqn: ?; simpl; eauto.
+                rewrite getDistinct; eauto.
+                intro; subst; generalize (P3 _ (eq_refl _)); omega.
+                intros.
+                destruct (peekD xenv6) eqn: foo; simpl; eauto.
+                admit.
+                admit.
+                destruct (peekD xenv6) eqn: ?; simpl; eauto.
+                rewrite getDistinct; eauto.
+                intro; subst; generalize (P3 _ (eq_refl _)); omega.
+                intros.
+                destruct (peekD xenv6) eqn: foo; simpl; eauto.
+                admit.
+                admit.
+              * simpl; intuition eauto.
+              * eauto.
+            + subst; eauto using ValidDomainName_app.
+            + subst; eauto using chomp_label_length.
+            + eassumption.
+            + injections.
+              destruct (fun H => proj1 (Nat_decode_correct (P := fun _ => True) 8 (fun _ _ _ => I)) _ _ _ _ _ (transform b'' (transform b3 ext0)) Eeq H I Penc'') as [xenv4 [? xenv_eqv] ].
+              pose proof (proj1 Valid_data ""%string l ""%string (append_EmptyString_r _) label1_OK).
+              unfold pow2; simpl; omega.
+              destruct (fun H => proj1 (String_decode_correct (P := fun _ => True) (fun _ _ _ => I) (String.length l)) _ _ _ _ _ (transform b3 ext0) xenv_eqv H I Penc''') as [xenv6 [? xenv6_eqv] ]; eauto.
+              eapply IHn in Penc''''.
+              destruct Penc'''' as [xenv7 [? ?] ].
+              eexists; split.
+              rewrite Init.Wf.Fix_eq; auto using decode_body_monotone; simpl.
+              * match goal with
+                  |- context [Decode_w_Measure_le ?x ?y ?z ?m] =>
+                  pose proof (Decode_w_Measure_le_eq x y z m)
+                end.
+                simpl in H4;
+                  unfold decode_word at 1 in H4.
+                rewrite <- !transform_assoc in H4.
+                unfold decode_nat in H0.
+                apply DecodeBindOpt2_inv in H0;
+                  destruct H0 as [? [? [? [? ?] ] ] ]; injections; subst.
+                unfold decode_word in H0.
+                destruct (decode_word' 8 (transform b' (transform b'' (transform b3 ext0)))); simpl in H0; try discriminate; injections.
+                simpl in H4.
+                destruct (H4 _ _ _ (eq_refl _)).
+                rewrite <- !transform_assoc, H0; simpl; clear H0.
+                pose proof (proj1 Valid_data ""%string l _ (append_EmptyString_r _) label1_OK) as w';
+                  rewrite H8 in w'.
+                destruct (wlt_dec WO~1~0~1~1~1~1~1~1 x); simpl;
+                  try (elimtype False; apply WordFacts.wordToNat_lt in w; simpl in w; omega).
+                destruct (wlt_dec x WO~0~1~0~0~0~0~0~0); simpl.
+                destruct (weq x (wzero 8)).
+                subst; simpl in H8.
+                destruct l; simpl in H8; try discriminate.
+                unfold ValidLabel in label1_OK; simpl in label1_OK; omega.
+                match goal with
+                  |- context [Decode_w_Measure_lt ?x ?y ?z ?m] =>
+                  pose proof (Decode_w_Measure_lt_eq x y z m)
+                end.
+                simpl in H0; rewrite H8 in H1; rewrite H1 in H0.
+                destruct (H0 _ _ _ (eq_refl _)).
+                rewrite H5; simpl; rewrite H2.
+                destruct label1_OK as [H6' _]; rewrite H6';
+                  simpl.
+                reflexivity.
+                unfold not in n2.
+                assert (WO~0~1~0~0~0~0~0~0 < x \/ WO~0~1~0~0~0~0~0~0 = x)
+                  by (destruct (weq WO~0~1~0~0~0~0~0~0 x); eauto using le_neq_lt).
+                destruct H0; eauto.
+                generalize (WordFacts.wordToNat_lt H0); simpl; omega.
+                generalize (f_equal (@wordToNat 8) H0); simpl; omega.
+              * clear l_eq.
+                split. erewrite peek_correct; eauto.
+                destruct (peekD xenv) eqn: ?; simpl; intuition eauto.
+                apply add_correct_G; intuition eauto.
+                { unfold decode_nat in H0.
                   apply DecodeBindOpt2_inv in H0;
                     destruct H0 as [? [? [? [? ?] ] ] ]; injections; subst.
-                  unfold decode_word in H0.
-                  destruct (decode_word' 8 (transform b' (transform b'' (transform b3 ext0)))); simpl in H0; try discriminate; injections.
-                  simpl in H4.
-                  destruct (H4 _ _ _ (eq_refl _)).
-                  rewrite <- !transform_assoc, H0; simpl; clear H0.
-                  pose proof ((proj1 Valid_data) ""%string label1 _ (eq_refl _) label1_OK) as w';
-                    rewrite H8 in w'.
-                  destruct (wlt_dec WO~1~0~1~1~1~1~1~1 x); simpl;
-                    try (elimtype False;
-                         apply WordFacts.wordToNat_lt in w; simpl in w; omega).
-                  destruct (wlt_dec x WO~0~1~0~0~0~0~0~0); simpl.
-                  * destruct (weq x (wzero 8)).
-                    subst; simpl in H8.
-                    destruct label1; simpl in H8; try discriminate.
-                    unfold ValidLabel in label1_OK; simpl in label1_OK; omega.
-                    match goal with
-                      |- context [Decode_w_Measure_lt ?x ?y ?z ?m] =>
-                      pose proof (Decode_w_Measure_lt_eq x y z m)
-                    end.
-                    simpl in H0; rewrite H8 in H1; rewrite H1 in H0.
-                    destruct (H0 _ _ _ (eq_refl _)).
-                    rewrite H5; simpl; rewrite H2.
-                    destruct label1_OK as [H6' _]; rewrite H6';
-                      simpl.
-                    destruct (string_dec label2 ""); simpl;
-                      try reflexivity.
-                    generalize (proj2 Valid_data label1 label2 (eq_refl _)); intros;
-                    rewrite e in H6; intuition.
-                  * destruct n2.
-                    rewrite <- natToWord_wordToNat;
-                      rewrite <- (natToWord_wordToNat x).
-                    apply WordFacts.natToWord_wlt.
-                    simpl.
-                    apply Nomega.Nlt_in.
-                    rewrite Nnat.Nat2N.id; etransitivity; eauto.
-                    simpl. unfold BinPos.Pos.to_nat; simpl.
-                    omega.
-                    apply Nomega.Nlt_in.
-                    simpl. unfold BinPos.Pos.to_nat; simpl.
-                    omega.
-                    simpl; omega.
-                + split. 
-                  erewrite l_eq', peek_correct by eauto.
-                  apply add_correct_G; eauto.
-                  intuition.
-                  apply DecodeBindOpt2_inv in H0;
-                    destruct H0 as [? [? [? [? ?] ] ] ]; injections; subst.
-                  pose proof (decode_word_peek_distinct _ _ _ _ _ _ H0) as P.
-                  pose proof (decode_string_peek_distinct _ _ _ _ _ _ H1) as P'.
-                  eapply decode_word_add_ptr_OK in H0; eauto.
-                  eapply decode_string_add_ptr_OK in H1; eauto.
-                  unfold add_ptr_OK in *; simpl in *; revert addPeek_eq getDistinct IndependentCaches H2 H1 P P'; clear.
-                  generalize (transform b3 ext0); intro.
-                  revert xenv label2 xenv6 xenv7 ext0.
+                  eapply decode_word_add_ptr_OK with (env := env) (env' := env) in H0; eauto.
+                  eapply decode_string_add_ptr_OK with (env := env)  in H1; eauto.
+                  unfold add_ptr_OK in *; simpl in *; revert getDistinct IndependentCaches H2 H1.
+                  remember ""%string as s'; rewrite Heqs'; rewrite <- Heqs' at 1.
+                  generalize env; clear.
+                  generalize (transform b3 ext0) ; intro.
+                  revert xenv6 xenv7 ext0 s'.
                   eapply (@well_founded_induction _ _ well_founded_lt_b) with
                   (a := b); intros.
                   rewrite Coq.Init.Wf.Fix_eq in H2; auto using decode_body_monotone; simpl.
@@ -1001,186 +1292,58 @@ Section DomainName.
                     destruct H2 as [? [? [? [? ?] ] ] ]; injections; subst.
                   destruct (wlt_dec  WO~1~0~1~1~1~1~1~1 x0); simpl in H2.
                   * (* The decoded word was a pointer. *)
-                    symmetry in H2; apply DecodeBindOpt2_inv in H2;
-                      destruct H2 as [? [? [? [? ?] ] ] ]; injections; subst.
-                    match type of H3 with
+                    symmetry in H4; apply DecodeBindOpt2_inv in H4;
+                      destruct H4 as [? [? [? [? ?] ] ] ]; injections; subst.
+                    match type of H5 with
                     | context [getD ?env' ?w] => destruct (getD env' w) eqn:getD_eq;
                                                    try discriminate
                     end.
                     destruct s; try discriminate; injections.
-                    eapply Decode_w_Measure_le_eq' in H2.
-                    eapply Decode_w_Measure_le_eq' in H0.
-                    unfold decode_word in H0.
-                    destruct (decode_word' 8 x); simpl in *; try discriminate; injections.
-                    unfold decode_word in H2.
-                    destruct (decode_word' 8 (projT1 x2)); simpl in *; try discriminate; injections.
-                    repeat match type of H2 with
-                           | context [dequeue_opt ?b] => destruct (dequeue_opt b) as [ [? ?] | ]; simpl in H2; try discriminate
-                           end.
+                    eapply Decode_w_Measure_le_eq' in H2; eauto.
+                    eapply decode_word_add_ptr_OK with (env := env) (env' := env) in H2; eauto.
+                    eapply Decode_w_Measure_le_eq' in H4; eauto.
+                    eapply decode_word_add_ptr_OK with (env := env) in H4; eauto.
+                  * destruct (wlt_dec x0 WO~0~1~0~0~0~0~0~0); simpl in H4; try discriminate.
+                    destruct (weq x0 (wzero 8)); simpl in H4.
                     injections.
-                    rewrite !IndependentCaches; eauto.
-                    repeat match type of H2 with
-                           | context [dequeue_opt ?b] => destruct (dequeue_opt b) as [ [? ?] | ]; simpl in H2; try discriminate
-                           end.
-                    injections.
-                    rewrite !IndependentCaches; eauto.
-                    eauto.
-                    eauto.
-                  * destruct (wlt_dec x0 WO~0~1~0~0~0~0~0~0); simpl in H2; try discriminate.
-                    destruct (weq x0 (wzero 8)); simpl in H2.
-                    injections.
-                    eapply Decode_w_Measure_le_eq' in H0.
-                    unfold decode_word in H0.
-                    destruct (decode_word' 8 x); simpl in *; try discriminate; injections.
-                    rewrite IndependentCaches; eauto.
-                    eauto.
-                    symmetry in H2; apply DecodeBindOpt2_inv in H2;
-                      destruct H2 as [? [? [? [? ?] ] ] ]; injections; subst.
-                    destruct (index 0 "." x4); simpl in H3; try discriminate.
-                    match type of H3 with
+                    eapply Decode_w_Measure_le_eq' in H2; eauto.
+                    eapply decode_word_add_ptr_OK with (env := env) (env' := env) in H2; eauto.
+                    eapply Decode_w_Measure_le_eq' in H2; eauto.
+                    (*eapply decode_word_add_ptr_OK in H2; eauto. *)
+                    symmetry in H4; apply DecodeBindOpt2_inv in H4;
+                      destruct H4 as [? [? [? [? ?] ] ] ]; injections; subst.
+                    destruct (index 0 "." x3); simpl in H5; try discriminate.
+                    match type of H5 with
                     | context [Fix well_founded_lt_b ?H' ?H0' ?H1' ?H2' ] =>
-                      destruct (Fix well_founded_lt_b H' H0' H1' H2') as [ [ [? ?] ?] | ] eqn:rec; simpl in H3;
+                      destruct (Fix well_founded_lt_b H' H0' H1' H2') as [ [ [? ?] ?] | ] eqn:rec; simpl in H5;
                         try discriminate
                     end.
-                    eapply Decode_w_Measure_le_eq' in H0; eauto.
-                    eapply Decode_w_Measure_lt_eq' in H2; eauto.
-                    pose proof (decode_word_peek_distinct _ _ _ _ _ _ H0) as P''.
-                    eapply decode_word_add_ptr_OK in H0; eauto.
-                    pose proof (decode_string_peek_distinct _ _ _ _ _ _ H2) as P'''.
-                    eapply decode_string_add_ptr_OK in H2; eauto.                    
-                    destruct (string_dec d ""); simpl in H3; injections;
+                    eapply Decode_w_Measure_lt_eq' in H4; eauto.
+                    (*eapply decode_string_add_ptr_OK in H4; eauto. *)
+                    destruct (string_dec d ""); simpl in H5; injections;
                       eapply H in rec; eauto using lt_B_trans.
-                    rewrite getDistinct; eauto.
-                    intro G; rewrite G in P'.
-                    eapply addPeek_eq in P; eauto.
-                    rewrite P'''.
-                    clear H0 H2; admit.
-                    clear H0 H2; admit.
-                    clear H0 H2; admit.
-                  * eauto.
-              + subst; eauto using ValidDomainName_app.
-              + subst; eauto using chomp_label_length.
-              + eassumption.
-              + injections.
-                  destruct (fun H => proj1 (Nat_decode_correct (P := fun _ => True) 8 (fun _ _ _ => I)) _ _ _ _ _ (transform b'' (transform b3 ext0)) Eeq H I Penc'') as [xenv4 [? xenv_eqv] ].
-                  pose proof (proj1 Valid_data ""%string l ""%string (append_EmptyString_r _) label1_OK).
-                simpl; omega.
-                destruct (fun H => proj1 (String_decode_correct (P := fun _ => True) (fun _ _ _ => I) (String.length l)) _ _ _ _ _ (transform b3 ext0) xenv_eqv H I Penc''') as [xenv6 [? xenv6_eqv] ]; eauto.
-                eapply IHn in Penc''''.
-                destruct Penc'''' as [xenv7 [? ?] ].
-                eexists; split.
-                rewrite Init.Wf.Fix_eq; auto using decode_body_monotone; simpl.
-                  * match goal with
-                      |- context [Decode_w_Measure_le ?x ?y ?z ?m] =>
-                      pose proof (Decode_w_Measure_le_eq x y z m)
-                    end.
-                    simpl in H4;
-                      unfold decode_word at 1 in H4.
-                    rewrite <- !transform_assoc in H4.
-                    unfold decode_nat in H0.
-                    apply DecodeBindOpt2_inv in H0;
-                      destruct H0 as [? [? [? [? ?] ] ] ]; injections; subst.
-                    unfold decode_word in H0.
-                    destruct (decode_word' 8 (transform b' (transform b'' (transform b3 ext0)))); simpl in H0; try discriminate; injections.
-                    simpl in H4.
-                    destruct (H4 _ _ _ (eq_refl _)).
-                    rewrite <- !transform_assoc, H0; simpl; clear H0.
-                    pose proof (proj1 Valid_data ""%string l _ (append_EmptyString_r _) label1_OK) as w';
-                    rewrite H8 in w'.
-                  destruct (wlt_dec WO~1~0~1~1~1~1~1~1 x); simpl;
-                    try (elimtype False; apply WordFacts.wordToNat_lt in w; simpl in w; omega).
-                  destruct (wlt_dec x WO~0~1~0~0~0~0~0~0); simpl.
-                  destruct (weq x (wzero 8)).
-                    subst; simpl in H8.
-                    destruct l; simpl in H8; try discriminate.
-                    unfold ValidLabel in label1_OK; simpl in label1_OK; omega.
-                    match goal with
-                      |- context [Decode_w_Measure_lt ?x ?y ?z ?m] =>
-                      pose proof (Decode_w_Measure_lt_eq x y z m)
-                    end.
-                    simpl in H0; rewrite H8 in H1; rewrite H1 in H0.
-                    destruct (H0 _ _ _ (eq_refl _)).
-                    rewrite H5; simpl; rewrite H2.
-                    destruct label1_OK as [H6' _]; rewrite H6';
-                      simpl.
-                    reflexivity.
-                    unfold not in n2.
-                    assert (WO~0~1~0~0~0~0~0~0 < x \/ WO~0~1~0~0~0~0~0~0 = x)
-                    by (destruct (weq WO~0~1~0~0~0~0~0~0 x); eauto using le_neq_lt).
-                    destruct H0; eauto.
-                    generalize (WordFacts.wordToNat_lt H0); simpl; omega.
-                    generalize (f_equal (@wordToNat 8) H0); simpl; omega.
-                  * clear l_eq.
-                    split. erewrite peek_correct; eauto.
-                    apply add_correct_G; intuition eauto.
-                    { unfold decode_nat in H0.
-                      apply DecodeBindOpt2_inv in H0;
-                        destruct H0 as [? [? [? [? ?] ] ] ]; injections; subst.
-                      eapply decode_word_add_ptr_OK in H0; eauto.
-                      eapply decode_string_add_ptr_OK in H1; eauto.                    
-                      unfold add_ptr_OK in *; simpl in *; revert getDistinct IndependentCaches H2 H1; clear.
-                      remember ""%string as s'; rewrite Heqs'; rewrite <- Heqs' at 1.
-                      clear Heqs'.
-                      generalize (transform b3 ext0) ; intro.
-                      revert xenv xenv6 xenv7 ext0 s'.
-                     eapply (@well_founded_induction _ _ well_founded_lt_b) with
-                     (a := b); intros.
-                     rewrite Coq.Init.Wf.Fix_eq in H2; auto using decode_body_monotone; simpl.
-                     apply DecodeBindOpt2_inv in H2;
-                       destruct H2 as [? [? [? [? ?] ] ] ]; injections; subst.
-                     destruct (wlt_dec  WO~1~0~1~1~1~1~1~1 x0); simpl in H2.
-                     * (* The decoded word was a pointer. *)
-                       symmetry in H4; apply DecodeBindOpt2_inv in H4;
-                         destruct H4 as [? [? [? [? ?] ] ] ]; injections; subst.
-                       match type of H5 with
-                       | context [getD ?env' ?w] => destruct (getD env' w) eqn:getD_eq;
-                                                      try discriminate
-                       end.
-                       destruct s; try discriminate; injections.
-                       eapply Decode_w_Measure_le_eq' in H2; eauto.
-                       eapply decode_word_add_ptr_OK in H2; eauto.
-                       eapply Decode_w_Measure_le_eq' in H4; eauto.
-                       eapply decode_word_add_ptr_OK in H4; eauto.
-                     * destruct (wlt_dec x0 WO~0~1~0~0~0~0~0~0); simpl in H4; try discriminate.
-                       destruct (weq x0 (wzero 8)); simpl in H4.
-                       injections.
-                       eapply Decode_w_Measure_le_eq' in H2; eauto.
-                       eapply decode_word_add_ptr_OK in H2; eauto.
-                       eapply Decode_w_Measure_le_eq' in H2; eauto.
-                       eapply decode_word_add_ptr_OK in H2; eauto.
-                       symmetry in H4; apply DecodeBindOpt2_inv in H4;
-                         destruct H4 as [? [? [? [? ?] ] ] ]; injections; subst.
-                       destruct (index 0 "." x3); simpl in H5; try discriminate.
-                       match type of H5 with
-                       | context [Fix well_founded_lt_b ?H' ?H0' ?H1' ?H2' ] =>
-                         destruct (Fix well_founded_lt_b H' H0' H1' H2') as [ [ [? ?] ?] | ] eqn:rec; simpl in H5;
-                           try discriminate
-                       end.
-                       eapply Decode_w_Measure_lt_eq' in H4; eauto.
-                       eapply decode_string_add_ptr_OK in H4; eauto.                    
-                       destruct (string_dec d ""); simpl in H5; injections;
-                         eapply H in rec; eauto using lt_B_trans.
-                       rewrite H0; eauto.
-                       clear H2 H4; admit.
-                       rewrite H0; eauto.
-                       clear H2 H4; admit.
-                    }
-                    eauto.
-                  * unfold ValidDomainName; split; intros.
-                    destruct pre; simpl in *; try discriminate.
-                    destruct label; simpl in *; try discriminate.
-                    omega.
-                    destruct pre; simpl in *; try discriminate.
-                  * simpl; omega.
-                  * eassumption.
-            }
+                    admit. (* rewrite H0; eauto. *)
+                    clear H2 H4; admit.
+                    admit. (* rewrite H0; eauto. *)
+                    clear H2 H4; admit.
+                }
+                eauto.
+              * unfold ValidDomainName; split; intros.
+                destruct pre; simpl in *; try discriminate.
+                destruct label; simpl in *; try discriminate.
+                omega.
+                destruct pre; simpl in *; try discriminate.
+              * simpl; omega.
+              * eassumption.
+          }
         }
       }
       destruct_ex; intuition; eauto. }
-      {
+    {
       unfold decode_DomainName, encode_DomainName_Spec;
-      intros env env' xenv' data bin;
-      revert env env' xenv' data.
+        intros env env' xenv' data bin;
+        revert env env' xenv' data.
+
       eapply (@well_founded_induction _ _ well_founded_lt_b) with
       (a := bin); intros.
       rewrite Coq.Init.Wf.Fix_eq in H2; auto using decode_body_monotone; simpl.
@@ -1207,7 +1370,7 @@ Section DomainName.
                  (fDom := [DomainName; CacheEncode])
                  (fCod := (B * CacheEncode)%type));
           unfold Frame.monotonic_function; simpl;
-          auto using encode_body_monotone.
+            auto using encode_body_monotone.
         intros; eapply encode_body_monotone.
         simpl; auto.
         rewrite get_correct in getD_eq; eauto.
@@ -1276,6 +1439,7 @@ Section DomainName.
           destruct (string_dec x6 ""); simpl in *;
             injections.
           { injection H5; intros; rewrite H14.
+            destruct (peekD env') eqn: ?; simpl in *; eauto.
             eapply P_OK; eauto.
             split.
             unfold ValidDomainName; split; intros.
@@ -1304,6 +1468,7 @@ Section DomainName.
             omega.
           }
           { injection H5; intros; rewrite H14.
+            destruct (peekD env') eqn: ?; simpl in *; eauto.
             eapply P_OK; eauto.
             split.
             eapply ValidDomainName_app'; eauto.
@@ -1338,17 +1503,17 @@ Section DomainName.
             apply (@PickComputes _ _ (x3, x6)); simpl; intuition eauto.
             subst x6; eauto.
             unfold ValidLabel.
-              split.
-              eauto.
-              destruct x3; simpl.
-              elimtype False; eapply NonEmpty_String_wordToNat; eauto.
-              omega.
-              rewrite H16, length_append; omega.
-              computes_to_econstructor; simpl.
-              unfold encode_nat_Spec;
-                rewrite H9, natToWord_wordToNat; eauto.
-              computes_to_econstructor; simpl; eauto.
-              computes_to_econstructor; simpl; eauto.
+            split.
+            eauto.
+            destruct x3; simpl.
+            elimtype False; eapply NonEmpty_String_wordToNat; eauto.
+            omega.
+            rewrite H16, length_append; omega.
+            computes_to_econstructor; simpl.
+            unfold encode_nat_Spec;
+              rewrite H9, natToWord_wordToNat; eauto.
+            computes_to_econstructor; simpl; eauto.
+            computes_to_econstructor; simpl; eauto.
           }
           { injection H5; intros; try subst data.
             destruct x3; simpl.
@@ -1384,58 +1549,52 @@ Section DomainName.
           intros; etransitivity; eauto.
           eapply WordFacts.wordToNat_lt in w0; simpl in w0; omega.
           rewrite H16 in x3_OK.
-            apply (index_correct3 _ (String.length pre)) in x3_OK.
-            elimtype False;
-              generalize x3_OK; clear.
-            { induction pre; simpl.
-              - unfold substring; destruct post; simpl; congruence.
-              - destruct pre; simpl.
-                unfold substring; destruct post; simpl; congruence.
-                auto.
-            }
-            congruence.
-            destruct x3; simpl.
-            elimtype False; eapply NonEmpty_String_wordToNat; eauto.
-            omega.
-            eapply ValidDomainName_app'; eauto.
-            unfold ValidLabel; split; eauto.
-            destruct x3; simpl; try omega.
-            elimtype False; eapply NonEmpty_String_wordToNat; eauto.
-            eapply WordFacts.wordToNat_lt in w; simpl in w; omega.
-            destruct (string_dec x6 ""); simpl in *; injection H5; intros;
-              subst xenv'; subst data.
-            erewrite peek_correct.
-            apply add_correct_G.
-            eauto.
-            admit.
-            eauto.
-            erewrite peek_correct.
-            apply add_correct_G.
-            eauto.
-            admit.
-            eauto.
-            apply lt_B_trans; eauto.
-            assumption.
-            assumption.
+          apply (index_correct3 _ (String.length pre)) in x3_OK.
+          elimtype False;
+            generalize x3_OK; clear.
+          { induction pre; simpl.
+            - unfold substring; destruct post; simpl; congruence.
+            - destruct pre; simpl.
+              unfold substring; destruct post; simpl; congruence.
+              auto.
+          }
+          congruence.
+          destruct x3; simpl.
+          elimtype False; eapply NonEmpty_String_wordToNat; eauto.
+          omega.
+          eapply ValidDomainName_app'; eauto.
+          unfold ValidLabel; split; eauto.
+          destruct x3; simpl; try omega.
+          elimtype False; eapply NonEmpty_String_wordToNat; eauto.
+          eapply WordFacts.wordToNat_lt in w; simpl in w; omega.
+          destruct (string_dec x6 ""); simpl in *; injection H5; intros;
+            subst xenv'; subst data.
+          erewrite peek_correct by eauto.
+          destruct (peekD env') eqn: ?; simpl in *; eauto.
+          apply add_correct_G.
+          eauto.
+          unfold add_ptr_OK; simpl.
+          destruct (getD x8 p) eqn: ?; auto.
+          eapply get_correct in Heqo; eauto.
+
+          admit.
+          erewrite peek_correct by eauto.
+          destruct (peekD env') eqn: ?; simpl in *; eauto.
+          apply add_correct_G.
+          eauto.
+          admit.
+          apply lt_B_trans; eauto.
+          assumption.
+          assumption.
     }
-      Grab Existential Variables.
-    admit.
-    admit.
-    admit.
-    admit.
-    admit.
-    admit.
-    clear; admit.
-    clear; admit.
-    clear; admit.
-    clear; admit.
-    clear; admit.
-    clear; admit.
-    clear; admit.
-    clear; admit.
-    clear; admit.
-    clear; admit.
-    clear; admit.
+    Grab Existential Variables.
+    econstructor.
+    auto.
+    econstructor.
+    econstructor.
+    econstructor.
+    assumption.
+    econstructor.
   Qed.
 
   Print Assumptions DomainName_decode_correct.
